Isabelle/Shelley/Ledger.thy
@@ -32,4 +32,25 @@ inductive ledger_sts :: "l_env \<Rightarrow> l_state \<Rightarrow> tx \<Rightarr
       if "(slot, tx) \<turnstile> dpstate \<rightarrow>\<^bsub>DELEGS\<^esub>{txcerts tx} dpstate'"
       and "(slot, pp, undefined, undefined, undefined) \<turnstile> utxo_st \<rightarrow>\<^bsub>UTXOW\<^esub>{tx} utxo_st'"
 
+text \<open> Ledger sequence rules \<close>
+
+text \<open>
+  NOTE:
+  \<^item> No state updates are performed in \<open>seq_ledger_base\<close> since all updates in the spec are not
+    related to the "preservation of value" property.
+\<close>
+inductive ledgers_sts :: "(slot \<times> p_params \<times> coin) \<Rightarrow> l_state \<Rightarrow> tx list \<Rightarrow> l_state \<Rightarrow> bool"
+  (\<open>_ \<turnstile> _ \<rightarrow>\<^bsub>LEDGERS\<^esub>{_} _\<close> [51, 0, 51] 50)
+  where
+    seq_ledger_base: "
+      (slot, pp, reserves) \<turnstile> ls \<rightarrow>\<^bsub>LEDGERS\<^esub>{[]} ls'"
+      if "((utxo, deps, fees, us), (ds, ps)) = ls"
+      and "us' = us"
+      and "ds' = ds"
+      and "ls' = ((utxo, deps, fees, us'), (ds', ps))"
+  | seq_ledger_ind: "
+      (slot, pp, reserves) \<turnstile> ls \<rightarrow>\<^bsub>LEDGERS\<^esub>{\<Gamma> @ [c]} ls''"
+      if "(slot, pp, reserves) \<turnstile> ls \<rightarrow>\<^bsub>LEDGERS\<^esub>{\<Gamma>} ls'"
+      and "(slot, length \<Gamma> - 1, pp, reserves) \<turnstile> ls' \<rightarrow>\<^bsub>LEDGER\<^esub>{c} ls''"
+
 end
